examples/Sugar2/Sugar2Script.sml
@@ -55,8 +55,6 @@ val S_BOOL_TRUE =
 (******************************************************************************
 * Set default parsing to natural numbers rather than integers 
 ******************************************************************************)
-val _ = intLib.deprecate_int();
-
 val S_REPEAT_BOOL_TRUE =
  store_thm
   ("S_REPEAT_BOOL_TRUE",
@@ -74,15 +72,15 @@ val S_REPEAT_BOOL_TRUE =
        THEN RES_TAC,
       Q.EXISTS_TAC `MAP (\l. [l]) w`
        THEN RW_TAC list_ss 
-             [EVERY_EL,CONCAT_MAP_SINGLETON,LENGTH_EL_MAP_SINGLETON,HD_EL_MAP]]);
+             [EVERY_EL,CONCAT_MAP_SINGLETON,LENGTH_EL_MAP_SINGLETON,
+              HD_EL_MAP]]);
 
 val FIRST_RISE_IMP =
- store_thm
-  ("FIRST_RISE_IMP",
-   ``FIRST_RISE M p c i ==>
-       (!j. j < i ==> ~B_SEM M (getL M (PATH_EL p j)) c) 
-       /\ 
-       B_SEM M (getL M (PATH_EL p i)) c``,
+ prove
+  (``FIRST_RISE M p c i ==>
+      (!j. j < i ==> ~B_SEM M (getL M (PATH_EL p j)) c) 
+      /\ 
+      B_SEM M (getL M (PATH_EL p i)) c``,
    REWRITE_TAC [FIRST_RISE_def]
     THEN ONCE_REWRITE_TAC[S_SEM_def]
     THEN SIMP_TAC list_ss 
@@ -90,9 +88,10 @@ val FIRST_RISE_IMP =
     THEN ONCE_REWRITE_TAC [EQ_SINGLETON]
     THEN RW_TAC std_ss []
     THENL
-     [ASSUM_LIST(fn thl => ASSUME_TAC(ONCE_REWRITE_RULE[el 3 thl](el 5 thl)))	
+     [ASSUM_LIST
+       (fn thl => ASSUME_TAC(ONCE_REWRITE_RULE[el 3 thl](el 5 thl)))	
        THEN IMP_RES_TAC(DECIDE ``j < i ==> i > 0``)
-       THEN IMP_RES_TAC MAP_PATH_SEG_APPLED_SINGLETON_IMP
+       THEN IMP_RES_TAC MAP_PATH_SEG_APPEND_SINGLETON_IMP0
        THEN ASSUM_LIST
               (fn thl 
                 => ASSUME_TAC
@@ -111,7 +110,91 @@ val FIRST_RISE_IMP =
        THEN POP_ASSUM
              (ASSUME_TAC o 
               SIMP_RULE list_ss [GSYM arithmeticTheory.ONE])
-       THEN IMP_RES_TAC(DECIDE``(n = 1) ==> (i + 1 = m + n) ==> j < i ==> j < m``)
+       THEN IMP_RES_TAC
+              (DECIDE``(n = 1) ==> (i + 1 = m + n) ==> j < i ==> j < m``)
+       THEN RES_TAC
+       THEN RW_TAC std_ss []
+       THEN ASSUM_LIST
+             (fn thl => ASSUME_TAC(REWRITE_RULE[LENGTH_MAP](el 2 thl)))
+       THEN POP_ASSUM
+             (fn th => 
+               ASSUME_TAC
+                (ISPEC 
+                  ``getL
+                     (M :'a # 'b # 'c # ('d -> bool) # ('e -> 'd -> bool))`` 
+                  (MATCH_MP EL_MAP th)))
+       THEN ASSUM_LIST
+             (fn thl => ASSUME_TAC(SIMP_RULE std_ss [el 1 thl](el 2 thl)))
+       THEN ASSUM_LIST
+             (fn thl  => 
+               ASSUME_TAC
+                (SIMP_RULE std_ss 
+                  [LENGTH_MAP,LENGTH_PATH_SEG_REC,PATH_SEG_def](el 4 thl)))
+       THEN IMP_RES_TAC(DECIDE``j < i - 1 - 0 + 1 ==> j <= i-1``)
+       THEN PROVE_TAC[EL_PATH_SEG0],
+      ASSUM_LIST(fn thl => ASSUME_TAC(ONCE_REWRITE_RULE[el 2 thl](el 4 thl)))
+       THEN ASSUM_LIST
+             (fn thl => 
+               ASSUME_TAC
+                (SIMP_RULE arith_ss 
+                  [LENGTH_MAP,LENGTH_APPEND,LENGTH,PATH_SEG_def,
+                   LENGTH_PATH_SEG_REC]
+                  (Q.AP_TERM `LENGTH` (el 1 thl))))
+       THEN Cases_on `i=0`
+       THENL
+        [RW_TAC arith_ss []
+          THEN IMP_RES_TAC(DECIDE``(0 + 1 = m + SUC 0) ==> (m = 0)``)
+          THEN FULL_SIMP_TAC arith_ss [LENGTH_NIL]
+          THEN FULL_SIMP_TAC list_ss [LENGTH,PATH_SEG_EL],
+         IMP_RES_TAC
+           (DECIDE
+             ``(i + 1 = m + SUC 0) ==> ~(i = 0) ==>  0 <= i-1 /\ i-1 < i``)
+          THEN IMP_RES_TAC(ISPEC ``p :'e path`` PATH_SEG_SPLIT)
+          THEN ASSUM_LIST
+                (fn thl =>
+                  ASSUME_TAC(SIMP_RULE arith_ss [el 1 thl] (el 6 thl)))
+          THEN IMP_RES_TAC(DECIDE``~(i = 0) ==> (i - 1 + 1 = i)``)
+          THEN POP_ASSUM
+                (fn th => 
+                  FULL_SIMP_TAC list_ss 
+                   [MAP_APPEND,th,PATH_SEG_EL,APPEND_CANCEL])]]);
+
+val NEXT_RISE_IMP =
+ prove
+  (``NEXT_RISE M p c (i,j) ==>
+      (!k. i <= k /\ k < j ==> ~B_SEM M (getL M (PATH_EL p k)) c) 
+      /\ 
+      (i <= j ==> B_SEM M (getL M (PATH_EL p j)) c)``,
+   REWRITE_TAC [NEXT_RISE_def]
+    THEN ONCE_REWRITE_TAC[S_SEM_def]
+    THEN SIMP_TAC list_ss 
+          [S_REPEAT_BOOL_TRUE,S_BOOL_TRUE,APPEND_INFIX_def,B_SEM_def]
+    THEN ONCE_REWRITE_TAC [EQ_SINGLETON]
+    THEN RW_TAC std_ss []
+    THENL
+     [ASSUM_LIST(fn thl => ASSUME_TAC(ONCE_REWRITE_RULE[el 4 thl](el 6 thl)))	
+       THEN IMP_RES_TAC(DECIDE ``i <= k ==> k < j ==> j > i``)
+       THEN IMP_RES_TAC MAP_PATH_SEG_APPEND_SINGLETON_IMP
+       THEN ASSUM_LIST
+              (fn thl 
+                => ASSUME_TAC
+                    (Q.AP_TERM 
+                     `LENGTH`
+                     (el 10 thl)))
+       THEN POP_ASSUM
+             (ASSUME_TAC o 
+              SIMP_RULE list_ss [LENGTH_MAP,LENGTH_PATH_SEG_REC,PATH_SEG_def])
+       THEN ASSUM_LIST
+              (fn thl 
+                => ASSUME_TAC
+                    (Q.AP_TERM 
+                     `LENGTH`
+                     (el 9 thl)))
+       THEN POP_ASSUM
+             (ASSUME_TAC o SIMP_RULE list_ss [GSYM arithmeticTheory.ONE])
+       THEN IMP_RES_TAC
+              (DECIDE``(n = 1) ==> (j - i + 1 = m + n) 
+                       ==> i <= k ==> k < j ==> k - i < m``)
        THEN RES_TAC
        THEN RW_TAC std_ss []
        THEN ASSUM_LIST(fn thl => ASSUME_TAC(REWRITE_RULE[LENGTH_MAP](el 2 thl)))
@@ -119,47 +202,192 @@ val FIRST_RISE_IMP =
              (fn th => 
                ASSUME_TAC
                 (ISPEC 
-                  ``getL (M :'a # 'b # 'c # ('d -> bool) # ('e -> 'd -> bool))`` 
+                  ``getL
+                     (M :'a # 'b # 'c # ('d -> bool) # ('e -> 'd -> bool))`` 
                   (MATCH_MP EL_MAP th)))
-       THEN ASSUM_LIST(fn thl => ASSUME_TAC(SIMP_RULE std_ss [el 1 thl](el 2 thl)))
        THEN ASSUM_LIST
-             (fn thl  => 
+             (fn thl => ASSUME_TAC(SIMP_RULE std_ss [el 1 thl](el 2 thl)))
+       THEN ASSUM_LIST
+             (fn thl  =>
                ASSUME_TAC
-                (SIMP_RULE std_ss [LENGTH_MAP,LENGTH_PATH_SEG_REC,PATH_SEG_def](el 4 thl)))
-       THEN IMP_RES_TAC(DECIDE``j < i - 1 - 0 + 1 ==> j <= i-1``)
-       THEN PROVE_TAC[EL_MAP_PATH_SEG],
-      ASSUM_LIST(fn thl => ASSUME_TAC(ONCE_REWRITE_RULE[el 2 thl](el 4 thl)))	
+                (SIMP_RULE std_ss [LENGTH_MAP,LENGTH_PATH_SEG](el 4 thl)))
+       THEN IMP_RES_TAC(DECIDE``i <= k ==> k < j ==>  k <= j - 1``)
+       THEN PROVE_TAC[EL_PATH_SEG],
+      ASSUM_LIST(fn thl => ASSUME_TAC(ONCE_REWRITE_RULE[el 3 thl](el 5 thl)))	
        THEN ASSUM_LIST
              (fn thl => 
                ASSUME_TAC
                 (SIMP_RULE arith_ss 
-                  [LENGTH_MAP,LENGTH_APPEND,LENGTH,PATH_SEG_def,LENGTH_PATH_SEG_REC]
+                  [LENGTH_MAP,LENGTH_APPEND,LENGTH,PATH_SEG_def,
+                   LENGTH_PATH_SEG_REC]
                   (Q.AP_TERM `LENGTH` (el 1 thl))))
-       THEN Cases_on `i=0`
+       THEN Cases_on `i=j`
        THENL
         [RW_TAC arith_ss []
-          THEN IMP_RES_TAC(DECIDE``(0 + 1 = m + SUC 0) ==> (m = 0)``)
+          THEN IMP_RES_TAC(DECIDE``(i - i + 1 = m + SUC 0) ==> (m = 0)``)
           THEN FULL_SIMP_TAC arith_ss [LENGTH_NIL]
           THEN RW_TAC arith_ss []
           THEN FULL_SIMP_TAC list_ss [LENGTH,PATH_SEG_EL],
-         IMP_RES_TAC(DECIDE``(i + 1 = m + SUC 0) ==> ~(i = 0) ==>  0 <= i-1 /\ i-1 < i``)
+         IMP_RES_TAC
+          (DECIDE``(j - i + 1 = m + SUC 0) 
+                   ==> ~(i = j) ==> i <= j ==>  i <= j-1 /\ j-1 < j``)
           THEN IMP_RES_TAC(ISPEC ``p :'e path`` PATH_SEG_SPLIT)
+          THEN POP_ASSUM(K ALL_TAC)
           THEN ASSUM_LIST
                 (fn thl =>
                   ASSUME_TAC(SIMP_RULE arith_ss [el 1 thl] (el 6 thl)))
-          THEN IMP_RES_TAC(DECIDE``~(i = 0) ==> (i - 1 + 1 = i)``)
+          THEN IMP_RES_TAC(DECIDE``j-1 < j ==> (j - 1 + 1 = j)``)
           THEN POP_ASSUM
-                (fn th => FULL_SIMP_TAC list_ss [MAP_APPEND,th,PATH_SEG_EL,APPEND_CANCEL])]]);
+                (fn th => FULL_SIMP_TAC list_ss 
+                  [MAP_APPEND,th,PATH_SEG_EL,APPEND_CANCEL])]]);
 
-(* To be proved (needs i>0 for <== direction?)
-val FIRST_RISE =
+val EL_MAP_COR =
  prove
-  (``FIRST_RISE M p c i = 
-       (!j. j < i ==> ~B_SEM M (getL M (PATH_EL p j)) c) 
-       /\ 
-       B_SEM M (getL M (PATH_EL p i)) c``,
-*)
+  (``!f. n < LENGTH l ==> (EL n (MAP f l) = f (EL n l))``,
+   RW_TAC std_ss [EL_MAP]);
 
+val FIRST_RISE_REVIMP =
+ prove
+  (``(!j. j < i ==> ~B_SEM M (getL M (PATH_EL p j)) c) 
+     /\ B_SEM M (getL M (PATH_EL p i)) c
+     ==>
+     FIRST_RISE M p c i``,
+   REWRITE_TAC [FIRST_RISE_def]
+    THEN ONCE_REWRITE_TAC[S_SEM_def]
+    THEN RW_TAC list_ss 
+          [S_REPEAT_BOOL_TRUE,S_BOOL_TRUE,APPEND_INFIX_def,B_SEM_def]
+    THEN Cases_on `i`
+     THENL
+      [Q.EXISTS_TAC `[]` THEN Q.EXISTS_TAC `MAP (getL M) (PATH_SEG p (0,0))` 
+        THEN RW_TAC list_ss [PATH_SEG_EL],
+      Q.EXISTS_TAC `MAP (getL M) (PATH_SEG p (0,n))`
+        THEN Q.EXISTS_TAC `MAP (getL M) (PATH_SEG p (SUC n,SUC n))` 
+        THEN RW_TAC list_ss []
+        THENL
+         [RW_TAC arith_ss [GSYM MAP_APPEND]
+           THEN REWRITE_TAC
+                 [SIMP_RULE arith_ss 
+                   [GSYM arithmeticTheory.ADD1] 
+                   (Q.SPECL[`p`,`n`,`0`,`SUC n`]PATH_SEG_SPLIT)],
+          POP_ASSUM
+            (ASSUME_TAC o 
+             SIMP_RULE arith_ss 
+              [PATH_SEG_def,PATH_SEG_REC_def,LENGTH_PATH_SEG_REC])
+           THEN FULL_SIMP_TAC std_ss [GSYM arithmeticTheory.ADD1]
+           THEN RES_TAC
+           THEN IMP_RES_TAC(DECIDE ``m < SUC n ==> m <= n``)
+           THEN IMP_RES_TAC
+                 (ISPECL[``i':num``,``n:num``,``p :'e path``] EL_PATH_SEG0)
+           THEN ASSUME_TAC
+                 (SIMP_RULE arith_ss [] 
+                   ((ISPECL[``0``,``n:num``,``p :'e path``] LENGTH_PATH_SEG)))
+           THEN IMP_RES_TAC(DECIDE ``(m = n+1) ==> i <= n ==> i < m``)
+           THEN IMP_RES_TAC
+                  (ISPECL
+                    [``getL
+                        (M :'a # 'b # 'c # ('d -> bool) # ('e -> 'd -> bool))``]
+                    EL_MAP_COR)
+           THEN RW_TAC std_ss [],
+          Q.EXISTS_TAC `getL M (PATH_EL p (SUC n))`          
+           THEN RW_TAC list_ss [PATH_SEG_EL]]]);
+
+
+val FIRST_RISE =
+ store_thm
+  ("FIRST_RISE",
+   ``FIRST_RISE M p c i =
+      (!j. j < i ==> ~B_SEM M (getL M (PATH_EL p j)) c) 
+      /\ 
+      B_SEM M (getL M (PATH_EL p i)) c``,
+   PROVE_TAC[FIRST_RISE_IMP, FIRST_RISE_REVIMP]);
+
+val FIRST_RISE_TRUE =
+ store_thm
+  ("FIRST_RISE_TRUE",
+   ``FIRST_RISE M p B_TRUE i = (i = 0)``,
+   RW_TAC std_ss [FIRST_RISE,L_def,B_SEM_def]
+    THEN EQ_TAC
+    THEN ZAP_TAC std_ss [intLib.COOPER_PROVE``(!j. ~(j < i)) = (i=0)``]);
+
+val NEXT_RISE_REVIMP =
+ prove
+  (``i <= j                                                       /\
+     (!k. i <= k /\ k < j ==> ~B_SEM M (getL M (PATH_EL p k)) c)  /\ 
+     B_SEM M (getL M (PATH_EL p j)) c  
+     ==>
+     NEXT_RISE M p c (i,j)``,
+   REWRITE_TAC [NEXT_RISE_def]
+    THEN ONCE_REWRITE_TAC[S_SEM_def]
+    THEN RW_TAC list_ss 
+          [S_REPEAT_BOOL_TRUE,S_BOOL_TRUE,APPEND_INFIX_def,B_SEM_def]
+    THEN Cases_on `i=j`
+     THENL
+      [RW_TAC std_ss []
+        THEN Q.EXISTS_TAC `[]` 
+        THEN Q.EXISTS_TAC `MAP (getL M) (PATH_SEG p (i,i))` 
+        THEN RW_TAC list_ss [PATH_SEG_EL],
+      Q.EXISTS_TAC `MAP (getL M) (PATH_SEG p (i,j-1))`
+        THEN Q.EXISTS_TAC `MAP (getL M) (PATH_SEG p (j,j))` 
+        THEN RW_TAC list_ss []
+        THENL
+         [RW_TAC arith_ss [GSYM MAP_APPEND]
+           THEN RW_TAC arith_ss [Q.SPECL[`p`,`j-1`,`i`,`j`]PATH_SEG_SPLIT],
+          POP_ASSUM
+            (ASSUME_TAC o 
+             SIMP_RULE arith_ss 
+              [PATH_SEG_def,PATH_SEG_REC_def,LENGTH_PATH_SEG_REC])
+           THEN IMP_RES_TAC
+                 (DECIDE``i <= j ==> ~(i = j) 
+                          ==> i' < j - (i + 1) + 1 ==> i <= i+i' /\ i+i' < j``)
+           THEN RES_TAC
+           THEN POP_ASSUM(K ALL_TAC)
+           THEN IMP_RES_TAC
+                  (DECIDE ``i <= i + i' ==> i + i' < j ==> i + i' <= j - 1``)
+           THEN IMP_RES_TAC
+                 (ISPECL[``i:num``,``i+i'``, ``j-1``,``p :'e path``]EL_PATH_SEG)
+           THEN FULL_SIMP_TAC std_ss [DECIDE ``i + i' - i = i'``]
+           THEN ASSUME_TAC
+                 (ISPECL[``i:num``,``j-1``,``p :'e path``]LENGTH_PATH_SEG)
+           THEN IMP_RES_TAC
+                 (DECIDE ``(m = j - 1 - i + 1) ==> i + i' < j ==> i' < m``)
+           THEN IMP_RES_TAC
+                  (ISPECL
+                    [``getL
+                        (M :'a # 'b # 'c # ('d -> bool) # ('e -> 'd -> bool))``]
+                    EL_MAP_COR)
+           THEN RW_TAC std_ss [],
+          Q.EXISTS_TAC `getL M (PATH_EL p j)`          
+           THEN RW_TAC list_ss [PATH_SEG_EL]]]);
+
+val NEXT_RISE =
+ store_thm
+  ("NEXT_RISE",
+   ``i <= j
+     ==>
+     (NEXT_RISE M p c (i,j) =
+       (!k. i <= k /\ k < j ==> ~B_SEM M (getL M (PATH_EL p k)) c)
+        /\ 
+        B_SEM M (getL M (PATH_EL p j)) c)``,
+   PROVE_TAC[NEXT_RISE_IMP, NEXT_RISE_REVIMP]);
+
+val NEXT_RISE_TRUE =
+ store_thm
+  ("NEXT_RISE_TRUE",
+   ``i <= j ==> (NEXT_RISE M p B_TRUE (i,j) = (i = j))``,
+   RW_TAC std_ss [NEXT_RISE,L_def,B_SEM_def]
+    THEN EQ_TAC
+    THENL
+     [RW_TAC arith_ss []
+       THEN POP_ASSUM(ASSUME_TAC o SIMP_RULE arith_ss [] o SPEC ``i:num``)
+       THEN DECIDE_TAC,
+      intLib.COOPER_TAC]);
+
+val NEXT_RISE_TRUE_EXISTS =
+ prove
+  (``?k. NEXT_RISE M p B_TRUE (j,k)``,
+   Q.EXISTS_TAC `j`
+    THEN RW_TAC std_ss 
+     [SIMP_RULE arith_ss [] (Q.SPECL[`p`,`j`,`j`](GEN_ALL NEXT_RISE_TRUE))]);
 
 (******************************************************************************
 * US_SEM M w r means "w is in the language of r" in the unclocked semantics
@@ -190,52 +418,140 @@ val US_SEM_def =
    (US_SEM M w (S_REPEAT r) = 
      ?wlist. (w = CONCAT wlist) /\ EVERY (\w. US_SEM M w r) wlist)`;
 
+
+(******************************************************************************
+* UF_SEM M p f means "p |= f"  in the unclocked semantics
+* (F_WEAK_IMP case unfolded to make totality proof go through)
+******************************************************************************)
+val UF_SEM_def =
+ Define
+   `(UF_SEM M p (F_BOOL b) = 
+      B_SEM M (L M (PATH_EL p 0)) b)
+    /\
+    (UF_SEM M p (F_NOT f) = 
+      ~(UF_SEM M p f)) 
+    /\
+    (UF_SEM M p (F_AND(f1,f2)) = 
+      UF_SEM M p f1 /\ UF_SEM M p f2)
+    /\
+    (UF_SEM M p (F_NEXT f) = 
+      (IS_FINITE_PATH p ==> PATH_LENGTH p > 1) /\
+       UF_SEM M (RESTN p 1) f)
+    /\
+    (UF_SEM M p (F_UNTIL(f1,f2)) = 
+      ?k. (* (IS_FINITE_PATH p ==> k < PATH_LENGTH p) /\ deleted for proof *)
+          UF_SEM M (RESTN p k) f2              /\
+          !j. j < k ==> UF_SEM M (RESTN p j) f1)
+    /\
+    (UF_SEM M p (F_SUFFIX_IMP(r,f)) = 
+      !j. US_SEM M (LHAT M (PATH_SEG p (0,j))) r
+          ==>
+          UF_SEM M (RESTN p j) f)
+    /\
+    (UF_SEM M p (F_STRONG_IMP(r1,r2)) = 
+      !j. US_SEM M (LHAT M (PATH_SEG p (0,j))) r1
+          ==>
+          ?k. US_SEM M (LHAT M (PATH_SEG p (j,k))) r2)
+    /\
+    (UF_SEM M p (F_WEAK_IMP(r1,r2)) = 
+(*     UF_SEM M p (F_STRONG_IMP(r1,r2))     *)
+       (!j. US_SEM M (LHAT M (PATH_SEG p (0,j))) r1
+          ==>
+          ?k. US_SEM M (LHAT M (PATH_SEG p (j,k))) r2)
+       \/
+       !j. US_SEM M (LHAT M (PATH_SEG p (0,j))) r1 ==>
+           (?k. US_SEM M (LHAT M (PATH_SEG p (j,k))) r2) \/
+           !k. (IS_FINITE_PATH p ==> k < PATH_LENGTH p)
+               ==> ?w. US_SEM M (LHAT M (PATH_SEG p (j,k)) <> w) r2)  
+    /\
+    (UF_SEM M p (F_ABORT (f,b)) =
+      UF_SEM M p f 
+      \/
+      ?j p'. UF_SEM M (RESTN p j) (F_BOOL b) /\ 
+             UF_SEM M (PATH_CAT(PATH_SEG p (0,j-1),p')) f)`;
+
+(******************************************************************************
+* UF_SEM M p f means "p |= f"  in the unclocked semantics
+* Derivation of folded equation
+******************************************************************************)
+val UF_SEM =
+ store_thm
+  ("UF_SEM",
+   ``(UF_SEM M p (F_BOOL b) = 
+       B_SEM M (L M (PATH_EL p 0)) b)
+     /\
+     (UF_SEM M p (F_NOT f) = 
+       ~(UF_SEM M p f)) 
+     /\
+     (UF_SEM M p (F_AND(f1,f2)) = 
+       UF_SEM M p f1 /\ UF_SEM M p f2)
+     /\
+     (UF_SEM M p (F_NEXT f) = 
+       (IS_FINITE_PATH p ==> PATH_LENGTH p > 1) /\
+        UF_SEM M (RESTN p 1) f)
+     /\
+     (UF_SEM M p (F_UNTIL(f1,f2)) = 
+       ?k. (* (IS_FINITE_PATH p ==> k < PATH_LENGTH p) /\ deleted for proof *)
+           UF_SEM M (RESTN p k) f2              /\
+           !j. j < k ==> UF_SEM M (RESTN p j) f1)
+     /\
+     (UF_SEM M p (F_SUFFIX_IMP(r,f)) = 
+       !j. US_SEM M (LHAT M (PATH_SEG p (0,j))) r
+           ==>
+           UF_SEM M (RESTN p j) f)
+     /\
+     (UF_SEM M p (F_STRONG_IMP(r1,r2)) = 
+       !j. US_SEM M (LHAT M (PATH_SEG p (0,j))) r1
+           ==>
+           ?k. US_SEM M (LHAT M (PATH_SEG p (j,k))) r2)
+     /\
+    (UF_SEM M p (F_WEAK_IMP(r1,r2)) = 
+       UF_SEM M p (F_STRONG_IMP(r1,r2))   
+       \/
+       !j. US_SEM M (LHAT M (PATH_SEG p (0,j))) r1 ==>
+           (?k. US_SEM M (LHAT M (PATH_SEG p (j,k))) r2) \/
+           !k. (IS_FINITE_PATH p ==> k < PATH_LENGTH p)
+               ==> ?w. US_SEM M (LHAT M (PATH_SEG p (j,k)) <> w) r2)  
+     /\
+     (UF_SEM M p (F_ABORT (f,b)) =
+       UF_SEM M p f 
+       \/
+       ?j p'. UF_SEM M (RESTN p j) (F_BOOL b) /\ 
+              UF_SEM M (PATH_CAT(PATH_SEG p (0,j-1),p')) f)``,
+   SIMP_TAC std_ss [UF_SEM_def]);
+
 (******************************************************************************
 * S_CLOCK_FREE r means r contains no clocking statements
 ******************************************************************************)
-
 val S_CLOCK_FREE_def =
  Define
-  `(S_CLOCK_FREE (S_BOOL b) = T)
+  `(S_CLOCK_FREE (S_BOOL b)          = T)
    /\
-   (S_CLOCK_FREE (S_CAT(r1,r2)) = 
-     S_CLOCK_FREE r1 /\ S_CLOCK_FREE r2)
+   (S_CLOCK_FREE (S_CAT(r1,r2))      =  S_CLOCK_FREE r1 /\ S_CLOCK_FREE r2)
    /\
-   (S_CLOCK_FREE (S_FUSION(r1,r2)) = 
-     S_CLOCK_FREE r1 /\ S_CLOCK_FREE r2) 
+   (S_CLOCK_FREE (S_FUSION(r1,r2))   = S_CLOCK_FREE r1 /\ S_CLOCK_FREE r2) 
    /\
-   (S_CLOCK_FREE (S_OR(r1,r2)) = 
-     S_CLOCK_FREE r1 /\ S_CLOCK_FREE r2) 
+   (S_CLOCK_FREE (S_OR(r1,r2))       = S_CLOCK_FREE r1 /\ S_CLOCK_FREE r2) 
    /\
-   (S_CLOCK_FREE (S_RIG_AND(r1,r2)) = 
-     S_CLOCK_FREE r1 /\ S_CLOCK_FREE r2) 
+   (S_CLOCK_FREE (S_RIG_AND(r1,r2))  = S_CLOCK_FREE r1 /\ S_CLOCK_FREE r2) 
    /\
-   (S_CLOCK_FREE (S_FLEX_AND(r1,r2)) = 
-     S_CLOCK_FREE r1 /\ S_CLOCK_FREE r2) 
+   (S_CLOCK_FREE (S_FLEX_AND(r1,r2)) = S_CLOCK_FREE r1 /\ S_CLOCK_FREE r2) 
    /\
-   (S_CLOCK_FREE (S_REPEAT r) = 
-     S_CLOCK_FREE r)
+   (S_CLOCK_FREE (S_REPEAT r)        = S_CLOCK_FREE r)
    /\
-   (S_CLOCK_FREE (S_CLOCK v) = F)`;
+   (S_CLOCK_FREE (S_CLOCK v)         = F)`;
 
 (******************************************************************************
 * Proof that if S_CLOCK_FREE r then the unclocked semantics of
 * SEREs is the same as the clocked semantics with clock equal to T
 ******************************************************************************)
-
-val LENGTH1 =
- prove
-  (``(LENGTH l = 1) = ?x. l=[x]``,
-   EQ_TAC
-    THEN RW_TAC list_ss [LENGTH,LENGTH_NIL,LENGTH_CONS,arithmeticTheory.ONE]);
-
 val S_SEM_TRUE_LEMMA =
  prove
-  (``!p1 p2 p3 p4 p5 w r. 
+  (``!m1 m2 m3 m4 m5 w r. 
       S_CLOCK_FREE r
       ==>
-      (S_SEM (p1,p2,p3,p4,p5) w B_TRUE r =
-        US_SEM (p1,p2,p3,p4,p5) w r)``,
+      (S_SEM (m1,m2,m3,m4,m5) w B_TRUE r =
+        US_SEM (m1,m2,m3,m4,m5) w r)``,
    recInduct (fetch "-" "US_SEM_ind")
     THEN RW_TAC std_ss [S_SEM_def, US_SEM_def, S_CLOCK_FREE_def]
     THENL
@@ -260,5 +576,70 @@ val S_SEM_TRUE =
    Cases_on `M` THEN Cases_on `r'` THEN Cases_on `r''` THEN Cases_on `r'`
     THEN RW_TAC std_ss [ S_SEM_TRUE_LEMMA]);
 
+(******************************************************************************
+* F_CLOCK_FREE f means f contains no clocking statements
+******************************************************************************)
+val F_CLOCK_FREE_def =
+ Define
+  `(F_CLOCK_FREE (F_BOOL b)            = T)
+   /\
+   (F_CLOCK_FREE (F_NOT f)             = F_CLOCK_FREE f) 
+   /\
+   (F_CLOCK_FREE (F_AND(f1,f2))        = F_CLOCK_FREE f1 /\ F_CLOCK_FREE f2)
+   /\
+   (F_CLOCK_FREE (F_NEXT f)            = F_CLOCK_FREE f)
+   /\
+   (F_CLOCK_FREE (F_UNTIL(f1,f2))      = F_CLOCK_FREE f1 /\ F_CLOCK_FREE f2)
+   /\
+   (F_CLOCK_FREE (F_SUFFIX_IMP(r,f))   = F_CLOCK_FREE f /\ S_CLOCK_FREE r)
+   /\
+   (F_CLOCK_FREE (F_STRONG_IMP(r1,r2)) = S_CLOCK_FREE r1 /\ S_CLOCK_FREE r2)
+   /\
+   (F_CLOCK_FREE (F_WEAK_IMP(r1,r2))   = S_CLOCK_FREE r1 /\ S_CLOCK_FREE r2)
+   /\
+   (F_CLOCK_FREE (F_ABORT (f,b))       = F_CLOCK_FREE f)
+   /\
+   (F_CLOCK_FREE (F_WEAK_CLOCK v)      = F)
+   /\
+   (F_CLOCK_FREE (F_STRONG_CLOCK v)    = F)`;
+
+val INIT_TAC =
+ RW_TAC std_ss
+  [F_SEM_def,UF_SEM_def,F_CLOCK_FREE_def,FIRST_RISE_TRUE,RESTN_def,
+   DECIDE``0 < n-1 = n > 1``,DECIDE``n >= 0``,DECIDE``0 <= n``];
+
+val F_SEM_TRUE_LEMMA =
+ store_thm
+  ("F_SEM_TRUE_LEMMA",
+   ``!m1 m2 m3 m4 m5 p f. 
+      F_CLOCK_FREE f
+      ==>
+      (F_SEM (m1,m2,m3,m4,m5) p (STRONG_CLOCK B_TRUE) f =
+        UF_SEM (m1,m2,m3,m4,m5) p f)``,
+   recInduct (fetch "-" "UF_SEM_ind")
+    THEN REPEAT CONJ_TAC
+    THENL
+     [(* F_STRONG_CLOCK v16 *)
+      INIT_TAC,
+      (* F_WEAK_CLOCK v14 *)
+      INIT_TAC,
+      (* F_BOOL b *)
+      INIT_TAC,
+      (* F_NOT b *)
+      INIT_TAC,
+      (* F_AND (f1,f2) *)
+      INIT_TAC,
+      (* F_NEXT f *)
+      INIT_TAC,
+      (* F_UNTIL(f1,f2) f *)
+      INIT_TAC THEN RW_TAC std_ss [B_SEM_def],
+      (* F_SUFFIX_IMP f *)
+      INIT_TAC THEN RW_TAC std_ss [S_SEM_TRUE],
+      (* F_STRONG_IMP f *)
+      INIT_TAC THEN RW_TAC std_ss [S_SEM_TRUE],
+      (* F_WEAK_IMP f *)
+      INIT_TAC THEN RW_TAC std_ss [S_SEM_TRUE,NEXT_RISE_TRUE_EXISTS],
+      (* F_ABORT(f,b)) *)
+      INIT_TAC THEN RW_TAC std_ss [B_SEM_def]]);
 
 val _ = export_theory();
